examples/wysteria/sec_server.fst
@@ -1,5 +1,5 @@
 (*--build-config
-    options:--admit_fsi FStar.OrdSet --admit_fsi FStar.Seq --admit_fsi FStar.OrdMap --admit_fsi FStar.Set --admit_fsi Ffibridge --admit_fsi Runtime --admit_fsi FStar.IO --admit_fsi FStar.String --__temp_no_proj --admit_fsi FStar.Squash;
+    options:--admit_fsi FStar.OrdSet --admit_fsi FStar.Seq --admit_fsi FStar.OrdMap --admit_fsi FStar.Set --admit_fsi Ffibridge --admit_fsi Runtime --admit_fsi FStar.IO --admit_fsi FStar.String --admit_fsi FStar.Squash --__temp_no_proj  PSemantics --__temp_no_proj SecServer;
     variables:CONTRIB=../../contrib;
     other-files:classical.fst ext.fst set.fsi heap.fst st.fst all.fst seq.fsi seqproperties.fst ghost.fst squash.fsti listTot.fst ordset.fsi ordmap.fsi list.fst io.fsti string.fsi prins.fst ast.fst ffibridge.fsi sem.fst psem.fst $CONTRIB/Platform/fst/Bytes.fst runtime.fsi print.fst ckt.fst crypto.fst interpreter.fst
  --*)
@@ -66,15 +66,20 @@ type psmap = ordmap prins psmap_v ps_cmp
 type psmap_ref_t =
   | Mk_ref: r:ref (ordmap prins psmap_v ps_cmp) -> psmap_ref_t
 
+val r_of_ref: x:psmap_ref_t -> Tot (ref (ordmap prins psmap_v ps_cmp))
+let r_of_ref = function
+  | Mk_ref r -> r
+
 (* private *)
 let psmap_ref = Mk_ref (alloc (OrdMap.empty #prins #psmap_v #ps_cmp))
 
 (* call interpreter step_star on the input config *)
 val do_sec_comp':
-  c:config -> ML (c':config{is_sterminal c'} & (sstep_star c c'))
+  c:config -> ML (d:(c':config & (sstep_star c c')){is_sterminal (dfst d)})
 let do_sec_comp' c =
-  let (| c_opt, h |) = step_star c in
+  let MkDTuple2 'a 'b c_opt h = step_star c in
   if is_sterminal c_opt then
+    let h = h in
     (| c_opt, h |)
   else
     failwith "Secure computation did not end in terminal state"
@@ -136,6 +141,10 @@ let init_sec_conf ps en_m x e =
   Conf Target (Mode Sec ps) [] (update_env (compose_envs_m ps en_m) x V_unit)
        (T_exp e) (hide [])
 
+(*
+ * TODO: Writing this proof without binding h makes create_pstep_star proof fast
+ * but then extraction fails
+ *)
 val get_sec_enter_step:
   ps:prins -> en_m:en_map{forall p. mem p ps = contains p en_m}
   -> red_m:redex_map{forall p.mem p ps = contains p red_m}
@@ -145,9 +154,9 @@ val get_sec_enter_step:
          pstep #ps (pi, (OrdMap.empty #prins #tconfig_sec #ps_cmp)) pi_enter)
 let get_sec_enter_step ps en_m red_m x e pi =
   let pi_enter = tstep_assec #ps (pi, (OrdMap.empty #prins #tconfig_sec #ps_cmp)) ps x e in
-  (| pi_enter,
-     P_sec_enter #ps (pi, (OrdMap.empty #prins #tconfig_sec #ps_cmp))
-                 ps x e (tstep_assec #ps (pi, (OrdMap.empty #prins #tconfig_sec #ps_cmp)) ps x e) |)
+  let h = P_sec_enter #ps (pi, (OrdMap.empty #prins #tconfig_sec #ps_cmp))
+                      ps x e (tstep_assec #ps (pi, (OrdMap.empty #prins #tconfig_sec #ps_cmp)) ps x e) in
+  (| pi_enter, h |)
 
 opaque val squash_pstep_star:
   ps:prins -> pi_init:protocol ps -> pi_final:protocol ps
@@ -185,7 +194,7 @@ val create_pstep_star:
   -> x:varname -> e:exp -> c_sec:config{is_sterminal c_sec}
   -> h:sstep_star (init_sec_conf ps en_m x e) c_sec
   -> pi:tpar ps{tpre_assec' ps ps pi x e en_m red_m}
-  -> Tot (pi_final:protocol ps{sec_comp_prop ps c_sec pi pi_final})
+  -> Tot (erased (pi_final:protocol ps{sec_comp_prop ps c_sec pi pi_final}))
 let create_pstep_star ps en_m red_m x e c_sec h pi =
   let pi_init = (pi, (OrdMap.empty #prins #tconfig_sec #ps_cmp)) in
   let en_m' = get_env_m #ps pi_init ps in
@@ -247,7 +256,7 @@ let create_pstep_star ps en_m red_m x e c_sec h pi =
   //squash_pstep_star ps pi_init pi_final h2;
 
   //let _ = cut (pstep_star #ps pi_init pi_final) in
-  pi_final
+  hide pi_final
 
 #reset-options
 
@@ -317,7 +326,7 @@ val build_pstep_star:
      SMTPatT (Good h)]
 let build_pstep_star ps en_m red_m x e c_sec h pi =
   let pi_final = create_pstep_star ps en_m red_m x e c_sec h pi in
-  let _ = cut (witness_build_pstep_star pi_final) in
+  let _ = cut (witness_build_pstep_star (reveal pi_final)) in
   ()
 
 val build_pstep_star_lemma:
@@ -379,7 +388,7 @@ let handle_connection c_in c_out =
     let R_assec #meta ps v = r in
     let (en, x, e) = get_en_b v in
 
-    let psmap_ref = Mk_ref.r psmap_ref in
+    let psmap_ref = r_of_ref psmap_ref in
 
     let ps', en_m, out_m, red_m =
       if contains ps !psmap_ref then
@@ -424,7 +433,7 @@ let handle_connection c_in c_out =
 
     if ps = ps' then
       let c_sec_init = Conf Target (Mode Sec ps) [] (update_env (compose_envs_m ps en_m) x V_unit) (T_exp e) (hide []) in
-      let (| c_sec, sstep_h |) = do_sec_comp' c_sec_init in
+      let MkDTuple2 'a 'b c_sec sstep_h = do_sec_comp' c_sec_init in
 
       let _ = cut (b2t (is_sterminal c_sec)) in
       let _ = admitP (Good sstep_h) in
