examples/wysteria/ckt.fst
@@ -1,6 +1,7 @@
 (*--build-config
-    options:--admit_fsi FStar.OrdSet --admit_fsi FStar.OrdMap --admit_fsi Ffibridge --admit_fsi FStar.Set --admit_fsi FStar.String --admit_fsi FStar.IO --admit_fsi Runtime --__temp_no_proj;
-    other-files:ghost.fst listTot.fst ordset.fsi ordmap.fsi classical.fst set.fsi heap.fst st.fst all.fst list.fst io.fsti string.fsi prins.fst ast.fst ffibridge.fsi sem.fst runtime.fsi print.fst
+    options:--admit_fsi FStar.OrdSet --admit_fsi FStar.OrdMap --admit_fsi Ffibridge --admit_fsi FStar.Set --admit_fsi FStar.String --admit_fsi FStar.IO --admit_fsi Runtime --admit_fsi FStar.Seq;
+    variables:CONTRIB=../../contrib;
+    other-files:classical.fst ext.fst set.fsi heap.fst st.fst all.fst seq.fsi seqproperties.fst ghost.fst listTot.fst ordset.fsi ordmap.fsi list.fst io.fsti string.fsi prins.fst ast.fst ffibridge.fsi sem.fst $CONTRIB/Platform/fst/Bytes.fst runtime.fsi print.fst
  --*)
 
 module Circuit
