examples/wysteria/theory.fst
@@ -1,5 +1,5 @@
 (*--build-config
-    options:--admit_fsi FStar.Set --admit_fsi FStar.OrdSet --admit_fsi FStar.OrdMap --admit_fsi Prins --admit_fsi Ffibridge --z3timeout 10 --__temp_no_proj;
+    options:--admit_fsi FStar.Set --admit_fsi FStar.OrdSet --admit_fsi FStar.OrdMap --admit_fsi Prins --admit_fsi Ffibridge --z3timeout 10 --__temp_no_proj PSemantics --__temp_no_proj Metatheory;
     other-files:ghost.fst listTot.fst set.fsi ordset.fsi ordmap.fsi constr.fst ext.fst classical.fst prins.fsi ast.fst ffibridge.fsi sem.fst psem.fst
  --*)
 
